src/AwsCryptographicMaterialProviders/Keyrings/RawRSAKeyring.dfy
@@ -1,0 +1,222 @@
+// Copyright Amazon.com Inc. or its affiliates. All Rights Reserved.
+// SPDX-License-Identifier: Apache-2.0
+
+include "../Keyring.dfy"
+include "../Materials.dfy"
+include "../AlgorithmSuites.dfy"
+include "../../StandardLibrary/StandardLibrary.dfy"
+include "../AlgorithmSuites.dfy"
+include "../../Crypto/Random.dfy"
+include "../../Crypto/RSAEncryption.dfy"
+include "../Materials.dfy"
+include "../../Util/UTF8.dfy"
+include "../../Util/Streams.dfy"
+include "../../Generated/AwsCryptographicMaterialProviders.dfy"
+include "../../../libraries/src/Collections/Sequences/Seq.dfy"
+
+
+  
+module
+  {:extern "Dafny.Aws.Crypto.MaterialProviders.RawRSAKeyring"}
+  MaterialProviders.RawRSAKeyring
+{
+  import opened StandardLibrary
+  import opened UInt = StandardLibrary.UInt
+  import opened Wrappers
+  import Aws.Crypto
+  import Keyring
+  import Materials
+  import opened AlgorithmSuites
+  import Random
+  import RSAEncryption
+  import UTF8
+  import Seq
+
+  type ValidRSAPublicKey = key: RSAEncryption.PublicKey | key.Valid()  witness *
+  type ValidRSAPrivateKey = key: RSAEncryption.PrivateKey | key.Valid() witness *
+
+  function method paddingSchemeToMinStrengthBits(
+    padding: RSAEncryption.PaddingMode
+  ): (strength: RSAEncryption.StrengthBits)
+    //Reverse of RSAEncryption.GetBtyes
+    ensures RSAEncryption.GetBytes(strength) == RSAEncryption.MinStrengthBytes(padding)
+  {
+    ((RSAEncryption.MinStrengthBytes(padding) * 8) - 7) as RSAEncryption.StrengthBits
+  }
+
+  //TODO :: What external method can we use to verify a pem is a pem?
+  //TODO :: Where should this method live? Probably in AwsCryptographicMaterialProviders
+  method importPrivateKey(
+    pem: seq<uint8>,
+    padding: RSAEncryption.PaddingMode
+  ) returns (res: Result<ValidRSAPrivateKey, string>)
+    requires |pem| > 0
+    requires RSAEncryption.GetBytes(paddingSchemeToMinStrengthBits(padding)) >= RSAEncryption.MinStrengthBytes(padding)
+    requires RSAEncryption.PEMGeneratedWithStrength(pem, paddingSchemeToMinStrengthBits(padding))
+    requires RSAEncryption.PEMGeneratedWithPadding(pem, padding)
+    ensures
+      res.Success?
+    ==>
+      && res.value.pem == pem
+      && res.value.strength >= paddingSchemeToMinStrengthBits(padding)
+      && res.value.padding == padding
+      && res.value.Valid()
+  {
+    var key := new RSAEncryption.PrivateKey(
+      pem := pem,
+      padding := padding,
+      strength := paddingSchemeToMinStrengthBits(padding)
+    );
+    return Success(key);
+  }
+
+  //TODO :: What external method can we use to verify a pem is a pem?
+  //TODO :: Where should calling said method live? Probably in AwsCryptographicMaterialProviders  
+  method importPublicKey(
+    pem: seq<uint8>,
+    padding: RSAEncryption.PaddingMode
+  ) returns (res: Result<ValidRSAPublicKey, string>)
+    requires |pem| > 0
+    requires RSAEncryption.GetBytes(paddingSchemeToMinStrengthBits(padding)) >= RSAEncryption.MinStrengthBytes(padding)
+    requires RSAEncryption.PEMGeneratedWithStrength(pem, paddingSchemeToMinStrengthBits(padding))
+    requires RSAEncryption.PEMGeneratedWithPadding(pem, padding)
+    ensures
+      res.Success?
+    ==>
+      && res.value.pem == pem
+      && res.value.strength >= paddingSchemeToMinStrengthBits(padding)
+      && res.value.padding == padding
+      && res.value.Valid()
+  {
+    var key := new RSAEncryption.PublicKey(
+      pem := pem,
+      padding := padding,
+      strength := paddingSchemeToMinStrengthBits(padding)
+    );
+    return Success(key);
+  }
+    
+  class RawRSAKeyring
+    extends Keyring.VerifiableInterface, Crypto.IKeyring
+  {
+    const keyNamespace: UTF8.ValidUTF8Bytes
+    const keyName: UTF8.ValidUTF8Bytes
+    const publicKey: Option<seq<uint8>>
+    const privateKey: Option<seq<uint8>>
+    const paddingScheme: RSAEncryption.PaddingMode
+
+    constructor (
+      namespace: UTF8.ValidUTF8Bytes,
+      name: UTF8.ValidUTF8Bytes,
+      publicKey: Option<seq<uint8>>,
+      privateKey: Option<seq<uint8>>,
+      paddingScheme: RSAEncryption.PaddingMode
+    )
+      requires |namespace| < UINT16_LIMIT
+      requires |name| < UINT16_LIMIT
+      ensures this.keyNamespace == namespace
+      ensures this.keyName == name
+      ensures this.paddingScheme == paddingScheme
+      ensures this.publicKey == publicKey
+      ensures this.privateKey == privateKey
+    {
+      this.keyNamespace := namespace;
+      this.keyName := name;
+      this.paddingScheme := paddingScheme;
+      this.publicKey := publicKey;
+      this.privateKey := privateKey;
+    }
+    
+    method OnEncrypt(input: Crypto.OnEncryptInput)
+      returns (res: Result<Crypto.OnEncryptOutput, string>)
+      ensures
+        res.Success?
+      ==>
+        && Materials.EncryptionMaterialsTransitionIsValid(
+          input.materials,
+          res.value.materials
+        )
+    {
+      :- Need(
+        this.publicKey.Some? && |this.publicKey.Extract()| > 0,
+        "A RawRSAKeyring without a public key cannot provide OnEncrypt"
+      );
+
+      var materials := input.materials;
+      var suite := GetSuite(materials.algorithmSuiteId);
+      
+      var newPlaintextDataKey :- Random.GenerateBytes(suite.encrypt.keyLength as int32);
+
+      var plaintextDataKey :=
+        if materials.plaintextDataKey.Some? && |materials.plaintextDataKey.Extract()| > 0
+        then materials.plaintextDataKey.value
+        else newPlaintextDataKey;
+      
+      var ciphertext :- RSAEncryption.EncryptExtern(
+        this.paddingScheme,
+        this.publicKey.Extract(),
+        plaintextDataKey
+      );
+        
+      var edk: Crypto.EncryptedDataKey := Crypto.EncryptedDataKey(
+        keyProviderId := this.keyNamespace,
+        keyProviderInfo := this.keyName,
+        ciphertext := ciphertext
+      );
+        
+      var r :- if materials.plaintextDataKey.None? then
+        Materials.EncryptionMaterialAddDataKey(materials, plaintextDataKey, [edk])
+      else
+        Materials.EncryptionMaterialAddEncryptedDataKeys(materials, [edk]);
+      return Success(Crypto.OnEncryptOutput(materials := r));      
+    }
+
+    method OnDecrypt(input: Crypto.OnDecryptInput)
+      returns (res: Result<Crypto.OnDecryptOutput, string>)
+      ensures res.Success?
+      ==>
+        && Materials.DecryptionMaterialsTransitionIsValid(
+          input.materials,
+          res.value.materials
+        )
+    {
+      :- Need(
+        this.privateKey.Some? && |this.privateKey.Extract()| > 0,
+        "A RawRSAKeyring without a private key cannot provide OnEncrypt"
+      );
+
+      var materials := input.materials;
+      :- Need(
+        Materials.DecryptionMaterialsWithoutPlaintextDataKey(materials),
+        "Keyring received decryption materials that already contain a plaintext data key."
+      );
+
+      var i := 0;
+      while i < |input.encryptedDataKeys|
+        invariant forall prevIndex :: 0 <= prevIndex < i ==> prevIndex < |input.encryptedDataKeys|
+      {
+        if ShouldDecryptEDK(input.encryptedDataKeys[i]) {
+          var edk := input.encryptedDataKeys[i];
+          var decryptResult := RSAEncryption.DecryptExtern(
+            this.paddingScheme,
+            this.privateKey.Extract(),
+            edk.ciphertext
+          );
+  
+          if decryptResult.Success? {
+            var r :- Materials.DecryptionMaterialsAddDataKey(materials, decryptResult.Extract());
+            return Success(Crypto.OnDecryptOutput(materials := r));
+          }
+        }
+        i := i + 1;
+      }
+      return Failure("Unable to decrypt data key: No Encrypted Data Keys found to match.");
+    }
+
+    predicate method ShouldDecryptEDK(edk: Crypto.EncryptedDataKey) {
+      && edk.keyProviderInfo == this.keyName
+      && edk.keyProviderId == this.keyNamespace
+      && |edk.ciphertext| > 0
+    }
+  }
+}
